WIP

NuBasicAbstractors.thy
@@ -25,12 +25,11 @@ section \<open>Abstractors for specification\<close>
 
 subsubsection \<open>Refinement\<close>
 
-definition NuRefine :: " ('a :: lrep, 'b) nu \<Rightarrow> 'b set \<Rightarrow> ('a, 'b) nu " (infixl "\<nuRefine>" 80)
-  where "N \<nuRefine> T = Nu (\<lambda>(p,x). x \<in> T \<and>(p \<nuLinkL> N \<nuLinkR> x))"
+definition NuRefine :: " ('a :: lrep, 'b) nu \<Rightarrow> 'b set \<Rightarrow> ('a, 'b) nu " (infixl "\<nuRefine>" 80) where "(N \<nuRefine> T) p x = (x \<in> T \<and>(p \<nuLinkL> N \<nuLinkR> x))"
 
-notation NuRefine (infixl "<where>" 10) and NuRefine (infixl "\<^bold>w\<^bold>h\<^bold>e\<^bold>r\<^bold>e" 60)
+notation NuRefine (infixl "<where>" 80) and NuRefine (infixl "\<^bold>w\<^bold>h\<^bold>e\<^bold>r\<^bold>e" 80)
 
-lemma [simp]: "p \<nuLinkL> N \<nuRefine> P \<nuLinkR> x \<longleftrightarrow> x \<in> P \<and> (p \<nuLinkL> N \<nuLinkR> x)" unfolding NuRefine_def by auto
+lemma [simp]: "p \<nuLinkL> N \<nuRefine> P \<nuLinkR> x \<longleftrightarrow> x \<in> P \<and> (p \<nuLinkL> N \<nuLinkR> x)" unfolding NuRefine_def Refining_ex by auto
 lemma [elim]: "x \<ratio> N \<nuRefine> P \<Longrightarrow> (x \<in> P \<Longrightarrow> x \<ratio> N \<Longrightarrow> C) \<Longrightarrow> C" unfolding Inhabited_def by auto
 lemma [\<nu>intro]: "(x \<in> P \<Longrightarrow> \<^bold>c\<^bold>a\<^bold>s\<^bold>t x \<tycolon> N \<longmapsto> Y \<^bold>m\<^bold>e\<^bold>a\<^bold>n\<^bold>w\<^bold>h\<^bold>i\<^bold>l\<^bold>e Q) \<Longrightarrow> \<^bold>c\<^bold>a\<^bold>s\<^bold>t x \<tycolon> N \<nuRefine> P \<longmapsto> Y \<^bold>m\<^bold>e\<^bold>a\<^bold>n\<^bold>w\<^bold>h\<^bold>i\<^bold>l\<^bold>e Q \<and>x \<in> P" unfolding Cast_def by auto
 lemma [\<nu>cast_overload E]: "\<^bold>c\<^bold>a\<^bold>s\<^bold>t x \<tycolon> (N \<^bold>w\<^bold>h\<^bold>e\<^bold>r\<^bold>e P) \<longmapsto> x \<tycolon> N \<^bold>m\<^bold>e\<^bold>a\<^bold>n\<^bold>w\<^bold>h\<^bold>i\<^bold>l\<^bold>e x \<in> P" unfolding Cast_def by auto
@@ -44,64 +43,72 @@ lemma [\<nu>intro]: "\<nu>CEqual N P eq \<Longrightarrow> \<nu>CEqual (N \<^bold
 lemma [\<nu>intro]: "\<nu>Ownership N ow \<Longrightarrow> \<nu>Ownership (N \<^bold>w\<^bold>h\<^bold>e\<^bold>r\<^bold>e S) ow" unfolding \<nu>Ownership_def by simp
 lemma [\<nu>intro]: "\<nu>ShrIdentical N sid \<Longrightarrow> \<nu>ShrIdentical (N \<^bold>w\<^bold>h\<^bold>e\<^bold>r\<^bold>e S) sid" unfolding \<nu>ShrIdentical_def by auto
 lemma [\<nu>intro]: "\<nu>Disposable \<tort_lbrace>x \<tycolon> N\<tort_rbrace> \<Longrightarrow> \<nu>Disposable \<tort_lbrace>x \<tycolon> (N \<^bold>w\<^bold>h\<^bold>e\<^bold>r\<^bold>e S)\<tort_rbrace>" unfolding \<nu>Disposable_def by simp
+lemma [\<nu>intro]: "\<^bold>p\<^bold>r\<^bold>e\<^bold>m\<^bold>i\<^bold>s\<^bold>e z \<in> S \<Longrightarrow> \<nu>Zero N z \<Longrightarrow> \<nu>Zero (N \<^bold>w\<^bold>h\<^bold>e\<^bold>r\<^bold>e S) z" unfolding \<nu>Zero_def Premise_def by simp
 
 subsubsection \<open>Down Lifting\<close>
 
 definition DownLift :: "(('a::lrep), 'b) nu \<Rightarrow> ('c \<Rightarrow> 'b) \<Rightarrow> ('a,'c) nu" (infixl "<down-lift>" 80)
-  where "DownLift N g = Nu (\<lambda>(p,x). p \<nuLinkL> N \<nuLinkR> g x)"
+  where "DownLift N g p x = (p \<nuLinkL> N \<nuLinkR> g x)"
 
-lemma [simp]: "p \<nuLinkL> N <down-lift> g \<nuLinkR> x \<longleftrightarrow> p \<nuLinkL> N \<nuLinkR> g x" unfolding DownLift_def by simp
+lemma [simp]: "p \<nuLinkL> N <down-lift> g \<nuLinkR> x \<longleftrightarrow> p \<nuLinkL> N \<nuLinkR> g x" unfolding DownLift_def Refining_ex by simp
 lemma [elim]: "x \<ratio> N <down-lift> g \<Longrightarrow> (g x \<ratio> N \<Longrightarrow> C) \<Longrightarrow> C" unfolding Inhabited_def by simp
 
 subsubsection \<open>Up Lifting\<close>
 
 definition UpLift :: "(('a::lrep), 'c) nu \<Rightarrow> ('c \<Rightarrow> 'b) \<Rightarrow> ('a,'b) nu" (infixl "<up-lift>" 80)
-  where "UpLift N f = Nu (\<lambda>(p,x). \<exists>y. f y = x \<and> (p \<nuLinkL> N \<nuLinkR> y))"
+  where "UpLift N f p x = (\<exists>y. f y = x \<and> (p \<nuLinkL> N \<nuLinkR> y))"
 
-lemma [simp]: "p \<nuLinkL> N <up-lift> f \<nuLinkR> x \<longleftrightarrow> (\<exists>y. (f y = x) \<and> (p \<nuLinkL> N \<nuLinkR> y))" unfolding UpLift_def by simp
+lemma [simp]: "p \<nuLinkL> N <up-lift> f \<nuLinkR> x \<longleftrightarrow> (\<exists>y. (f y = x) \<and> (p \<nuLinkL> N \<nuLinkR> y))" unfolding UpLift_def Refining_ex by simp
 lemma [elim]: "x \<ratio> N <up-lift> f \<Longrightarrow> (\<And>y. y \<ratio> N \<Longrightarrow> f y = x \<Longrightarrow> C) \<Longrightarrow> C" unfolding Inhabited_def by auto
-
-lemma [\<nu>intro]: "\<nu>Share "
 
 subsubsection \<open>Operator Some\<close>
 
 definition NuSome :: " ('a :: lrep, 'b) nu \<Rightarrow> ('a :: lrep, 'b set) nu " ("<some>")
-  where "NuSome N = Nu (\<lambda>(p,S). \<exists>x. x \<in> S \<and> (p \<nuLinkL> N \<nuLinkR> x))"
+  where "NuSome N p S = (\<exists>x. x \<in> S \<and> (p \<nuLinkL> N \<nuLinkR> x))"
 notation NuSome ("\<^bold>s\<^bold>o\<^bold>m\<^bold>e")
 
-lemma [simp]: "p \<nuLinkL> \<^bold>s\<^bold>o\<^bold>m\<^bold>e N \<nuLinkR> X \<longleftrightarrow> (\<exists>x. x \<in> X \<and> (p \<nuLinkL> N \<nuLinkR> x))" unfolding NuSome_def by auto
+lemma [simp]: "p \<nuLinkL> \<^bold>s\<^bold>o\<^bold>m\<^bold>e N \<nuLinkR> X \<longleftrightarrow> (\<exists>x. x \<in> X \<and> (p \<nuLinkL> N \<nuLinkR> x))" unfolding NuSome_def Refining_ex by auto
 lemma [elim]: "X \<ratio> ( \<^bold>s\<^bold>o\<^bold>m\<^bold>e N) \<Longrightarrow> (\<And>x. x \<in> X \<Longrightarrow> x \<ratio> N \<Longrightarrow> C) \<Longrightarrow> C" unfolding Inhabited_def by auto
 lemma [\<nu>intro]: "\<^bold>p\<^bold>r\<^bold>e\<^bold>m\<^bold>i\<^bold>s\<^bold>e X \<subseteq> X' \<Longrightarrow> \<^bold>c\<^bold>a\<^bold>s\<^bold>t X \<tycolon> (\<^bold>s\<^bold>o\<^bold>m\<^bold>e N) \<longmapsto> X' \<tycolon> (\<^bold>s\<^bold>o\<^bold>m\<^bold>e N)" unfolding Cast_def by (auto 2 3)
 lemma [\<nu>intro]: "\<^bold>p\<^bold>r\<^bold>e\<^bold>m\<^bold>i\<^bold>s\<^bold>e x \<in> X \<Longrightarrow> \<^bold>c\<^bold>a\<^bold>s\<^bold>t x \<tycolon> N \<longmapsto> X \<tycolon> (\<^bold>s\<^bold>o\<^bold>m\<^bold>e N)" unfolding Cast_def by auto
 lemma someI_\<nu>cast: "\<^bold>p\<^bold>a\<^bold>r\<^bold>a\<^bold>m X \<Longrightarrow> \<^bold>p\<^bold>r\<^bold>e\<^bold>m\<^bold>i\<^bold>s\<^bold>e x \<in> X \<Longrightarrow> \<^bold>c\<^bold>a\<^bold>s\<^bold>t x \<tycolon> N \<longmapsto> X \<tycolon> (\<^bold>s\<^bold>o\<^bold>m\<^bold>e N)" unfolding Cast_def by auto
 lemma someE_\<nu>cast[\<nu>cast_overload E]: "\<^bold>c\<^bold>a\<^bold>s\<^bold>t X \<tycolon> (\<^bold>s\<^bold>o\<^bold>m\<^bold>e N) \<longmapsto> (\<exists>*some. \<tort_lbrace>some \<tycolon> N \<tort_rbrace> \<addition> (some \<in> X))" unfolding Cast_def by auto
 
-subsubsection \<open>Pointer'\<close>
-
-definition "Pointer' = Pointer \<^bold>w\<^bold>h\<^bold>e\<^bold>r\<^bold>e {x. pred_owning within_mem x}"
-
-lemma [simp]: "memadr i' \<nuLinkL> Pointer' \<nuLinkR> i \<longleftrightarrow> (i' = i) \<and> pred_owning within_mem i" unfolding Pointer'_def by auto
-lemma [elim]: "z \<left_fish_tail> i \<ratio> Pointer' \<Longrightarrow> (within_mem i \<Longrightarrow> C) \<Longrightarrow> C" and [elim]: "\<down_fish_tail> \<ratio> Pointer' \<Longrightarrow> C \<Longrightarrow> C"
-  unfolding Inhabited_def by (simp add: memadr_exisits)+
 
 subsubsection \<open>Reference\<close>
 
-definition "Ref N = \<lbrace> Pointer' \<nuFusion> MemObj N \<rbrace>
-  <down-lift> (\<lambda>x. case x of (zp \<left_fish_tail> a \<R_arr_tail> z \<left_fish_tail> x) \<Rightarrow> (zp \<left_fish_tail> a, z \<left_fish_tail> a \<R_arr_tail> x) | (zp \<left_fish_tail> a \<R_arr_tail> \<down_fish_tail>) \<Rightarrow> (zp \<left_fish_tail> a, \<down_fish_tail>) | \<down_fish_tail> \<Rightarrow> (\<down_fish_tail>,\<down_fish_tail>))"
+type_synonym ('spc,'x) memref = "('spc memptr \<times> 'x memobj) tuple"
 
-lemma [simp]: "p \<nuLinkL> Ref N \<nuLinkR> (zp \<left_fish_tail> a \<R_arr_tail> z \<left_fish_tail> x) \<longleftrightarrow> p \<nuLinkL> \<lbrace> Pointer' \<nuFusion> MemObj N \<rbrace> \<nuLinkR> (zp \<left_fish_tail> a, z \<left_fish_tail> a \<R_arr_tail> x)"
-  and [simp]: "p \<nuLinkL> Ref N \<nuLinkR> (zp \<left_fish_tail> a \<R_arr_tail> \<down_fish_tail>) \<longleftrightarrow> p \<nuLinkL> \<lbrace> Pointer' \<nuFusion> MemObj N \<rbrace> \<nuLinkR> (zp \<left_fish_tail> a, \<down_fish_tail>)"
-  and [simp]: "p \<nuLinkL> Ref N \<nuLinkR> \<down_fish_tail> \<longleftrightarrow> p \<nuLinkL> \<lbrace> Pointer' \<nuFusion> MemObj N \<rbrace> \<nuLinkR> (\<down_fish_tail>, \<down_fish_tail>)"
+abbreviation "address_of_ref x \<equiv> (case x of _ \<left_fish_tail> a \<R_arr_tail> _ \<Rightarrow> a)"
+
+definition "Ref N = \<lbrace> Pointer \<nuFusion> MemObj N \<rbrace>
+  <down-lift> (\<lambda>x. case x of (zp \<left_fish_tail> a \<R_arr_tail> z \<left_fish_tail> x) \<Rightarrow> (zp \<left_fish_tail> a, z \<left_fish_tail> a \<R_arr_tail> x) | (zp \<left_fish_tail> a \<R_arr_tail> \<down_fish_tail>) \<Rightarrow> (zp \<left_fish_tail> a, \<down_fish_tail>) | \<down_fish_tail> \<Rightarrow> (\<down_fish_tail>,\<down_fish_tail>))
+  <where> {x. pred_owning (\<lambda>r. memadr_llty (adr_of_object r) = llty TYPE('b)) x}"
+  for N :: "('b::field, 'c) nu"
+
+lemma [simp]: "p \<nuLinkL> Ref N \<nuLinkR> (zp \<left_fish_tail> a \<R_arr_tail> z \<left_fish_tail> x) \<longleftrightarrow>
+    (memadr_llty a = llty TYPE('b)) \<and> (p \<nuLinkL> \<lbrace> Pointer \<nuFusion> MemObj N \<rbrace> \<nuLinkR> (zp \<left_fish_tail> a, z \<left_fish_tail> a \<R_arr_tail> x))"
+  and [simp]: "p \<nuLinkL> Ref N \<nuLinkR> (zp \<left_fish_tail> a \<R_arr_tail> \<down_fish_tail>) \<longleftrightarrow>
+    (memadr_llty a = llty TYPE('b)) \<and> (p \<nuLinkL> \<lbrace> Pointer \<nuFusion> MemObj N \<rbrace> \<nuLinkR> (zp \<left_fish_tail> a, \<down_fish_tail>))"
+  and [simp]: "p \<nuLinkL> Ref N \<nuLinkR> \<down_fish_tail> \<longleftrightarrow> p \<nuLinkL> \<lbrace> Pointer \<nuFusion> MemObj N \<rbrace> \<nuLinkR> (\<down_fish_tail>, \<down_fish_tail>)"
+  for N :: "('b::field, 'c) nu"
   unfolding Ref_def by simp+
 
-definition "share_ref z x = (case x of (zp \<left_fish_tail> a \<R_arr_tail> zx \<left_fish_tail> x) \<Rightarrow> (zp + z \<left_fish_tail> a \<R_arr_tail> zx + z \<left_fish_tail> x) | (zp \<left_fish_tail> a \<R_arr_tail> \<down_fish_tail>) \<Rightarrow> (zp + z \<left_fish_tail> a \<R_arr_tail> \<down_fish_tail>) | \<down_fish_tail> \<Rightarrow> \<down_fish_tail>)"
-lemma [simp]: "share_ref z (zp \<left_fish_tail> a \<R_arr_tail> zx \<left_fish_tail> x) = (zp + z \<left_fish_tail> a \<R_arr_tail> zx + z \<left_fish_tail> x)"
-  and [simp]: "share_ref z (zp \<left_fish_tail> a \<R_arr_tail> \<down_fish_tail>) = (zp + z \<left_fish_tail> a \<R_arr_tail> \<down_fish_tail>)"
-  and [simp]: "share_ref z \<down_fish_tail> = \<down_fish_tail>"
-  unfolding share_ref_def by auto
-lemma [\<nu>intro]: "\<nu>Share (Ref N) (\<lambda>x. T) share_ref"
-  unfolding \<nu>Share_def by (simp add: tuple_forall object_forall owning_forall memadr_forall memcon_forall)
+abbreviation "share_ref z x \<equiv> (case x of (zp \<left_fish_tail> a \<R_arr_tail> zx \<left_fish_tail> x) \<Rightarrow> (zp + z \<left_fish_tail> a \<R_arr_tail> zx + z \<left_fish_tail> x) | (zp \<left_fish_tail> a \<R_arr_tail> \<down_fish_tail>) \<Rightarrow> (zp + z \<left_fish_tail> a \<R_arr_tail> \<down_fish_tail>) | \<down_fish_tail> \<Rightarrow> \<down_fish_tail>)"
+lemma [\<nu>intro]: "\<nu>Share (Ref N) (\<lambda>x. T) share_ref" unfolding \<nu>Share_def by (simp add: lrep_exps)
 
+lemma [\<nu>intro]: "\<nu>Ownership N ow \<Longrightarrow> \<nu>ShrIdentical (Ref N) (rel_owning (rel_object (rel_owning (inv_imagep (=) ow))))"
+  unfolding \<nu>ShrIdentical_def \<nu>Ownership_def by (auto simp add: lrep_exps)
+
+abbreviation "ownership_ref ref \<equiv>
+  (case ref of zp \<left_fish_tail> a \<R_arr_tail> x \<Rightarrow> OWS_C (OWS_1 zp) (ownership x) | \<down_fish_tail> \<Rightarrow> OWS_C OWS_0 OWS_0)"
+lemma [\<nu>intro]: "\<nu>Ownership (Ref N) ownership_ref"
+  unfolding \<nu>Ownership_def by (simp add: lrep_exps)
+
+lemma [\<nu>intro]: "\<nu>Deprive (Ref N) (\<lambda>x. \<down_fish_tail>)" unfolding \<nu>Deprive_def by (simp add: lrep_exps)
+lemma [\<nu>intro]: "\<nu>CEqual (Ref N) (rel1_owning (\<lambda>x y. True)) (rel_owning (rel_object (\<lambda>x y. True)))"
+  unfolding \<nu>CEqual_def by (simp add: lrep_exps)
+lemma [\<nu>intro]: "\<nu>Zero (Ref N) \<down_fish_tail>" unfolding \<nu>Zero_def by simp
 
 (* section \<open>Others\<close>
 
